Implemented a reify/reflect system for FPLang.expr

leapfrog_project/float_lib.v
@@ -81,7 +81,6 @@ apply Zeq_bool_eq in H.
 unfold FLT_exp in H.
 rewrite Digits.Zpos_digits2_pos in H.
 set (d := Digits.Zdigits radix2 _) in *.
-Search Digits.Zdigits.
 (* should be provable from here . . ., but what a pain! *)
 Admitted.
 
@@ -100,7 +99,113 @@ Lemma mul_minusone_negate:
    Float32.mul (Float32.neg 1) x = Float32.neg x.
 Admitted.
 
+Require Import vcfloat.FPLang.
 
+Definition SterbenzSub32 := Float32.sub.
+Definition SterbenzSub := Float.sub.
+
+Definition placeholder32: AST.ident -> float32. intro. apply Float32.zero. Qed.
+
+Ltac reify_float_expr E :=
+ match E with
+ | placeholder32 ?i => constr:(@Var AST.ident Tsingle i)
+ | Float.of_single ?f => constr:(@Unop AST.ident (CastTo Tdouble None) f)
+ | Float.to_single ?f => constr:(@Unop AST.ident (CastTo Tsingle None) f)
+ | float32_of_Z ?n => constr:(@Const AST.ident Tsingle (float32_of_Z n))
+ | Float32.of_int ?i => constr:(@Const AST.ident Tsingle (float32_of_Z (Int.signed i)))
+ | Float32.of_intu ?i => constr:(@Const AST.ident Tsingle (float32_of_Z (Int.unsigned i)))
+ | Float32.of_long ?i => constr:(@Const AST.ident Tsingle (float32_of_Z (Int64.signed i)))
+ | Float32.of_longu ?i => constr:(@Const AST.ident Tsingle (float32_of_Z (Int64.unsigned i)))
+ | Float32.mul ?a ?b => let a' := reify_float_expr a in let b' := reify_float_expr b in 
+                                      constr:(@Binop AST.ident (Rounded2 MULT None) a' b')
+ | Float32.div ?a ?b => let a' := reify_float_expr a in let b' := reify_float_expr b in 
+                                      constr:(@Binop AST.ident (Rounded2 DIV None) a' b')
+ | Float32.add ?a ?b => let a' := reify_float_expr a in let b' := reify_float_expr b in 
+                                      constr:(@Binop AST.ident (Rounded2 PLUS None) a' b')
+ | Float32.sub ?a ?b => let a' := reify_float_expr a in let b' := reify_float_expr b in 
+                                      constr:(@Binop AST.ident (Rounded2 MINUS None) a' b')
+ | SterbenzSub32 ?a ?b => let a' := reify_float_expr a in let b' := reify_float_expr b in 
+                                      constr:(@Binop AST.ident SterbenzMinus a' b')
+ | Float32.neg ?a => let a' := reify_float_expr a in
+                                      constr:(@Unop AST.ident (Exact1 Opp) a')
+ | Float32.abs ?a => let a' := reify_float_expr a in
+                                      constr:(@Unop AST.ident (Exact1 Abs) a')
+ | float_of_Z ?n => constr:(@Const AST.ident Tsingle (float_of_Z n))
+ | Float.of_int ?i => constr:(@Const AST.ident Tsingle (float_of_Z (Int.signed i)))
+ | Float.of_intu ?i => constr:(@Const AST.ident Tsingle (float_of_Z (Int.unsigned i)))
+ | Float.of_long ?i => constr:(@Const AST.ident Tsingle (float_of_Z (Int64.signed i)))
+ | Float.of_longu ?i => constr:(@Const AST.ident Tsingle (float_of_Z (Int64.unsigned i)))
+ | Float.mul ?a ?b => let a' := reify_float_expr a in let b' := reify_float_expr b in 
+                                      constr:(@Binop AST.ident (Rounded2 MULT None) a' b')
+ | Float.div ?a ?b => let a' := reify_float_expr a in let b' := reify_float_expr b in 
+                                      constr:(@Binop AST.ident (Rounded2 DIV None) a' b')
+ | Float.add ?a ?b => let a' := reify_float_expr a in let b' := reify_float_expr b in 
+                                      constr:(@Binop AST.ident (Rounded2 PLUS None) a' b')
+ | Float.sub ?a ?b => let a' := reify_float_expr a in let b' := reify_float_expr b in 
+                                      constr:(@Binop AST.ident (Rounded2 MINUS None) a' b')
+ | SterbenzSub ?a ?b => let a' := reify_float_expr a in let b' := reify_float_expr b in 
+                                      constr:(@Binop AST.ident SterbenzMinus a' b')
+ | Float.neg ?a => let a' := reify_float_expr a in
+                                constr:(@Unop AST.ident (Exact1 Opp) a')
+ | Float.abs ?a => let a' := reify_float_expr a in
+                                constr:(@Unop AST.ident (Exact1 Abs) a')
+ | _ =>  let E' := eval red in E in reify_float_expr E'
+ | _ => fail 100 "could not reify" E
+ end.
+
+Ltac HO_reify_float_expr names E :=
+ lazymatch names with
+ | ?n :: ?names' =>
+             let Ev := constr:(E (placeholder32 n)) in 
+             HO_reify_float_expr names' Ev
+ | nil =>reify_float_expr E
+ end.
+
+Definition list_to_env (bindings: list (AST.ident * Values.val)) : (forall ty : type, AST.ident -> ftype ty) .
+pose (m :=   Maps.PTree_Properties.of_list bindings).
+intros ty i.
+destruct (type_eq_dec ty Tsingle); [ | destruct (type_eq_dec ty Tdouble)].
+{
+subst.
+destruct (Maps.PTree.get i m); [ | exact Float32.zero].
+destruct v; try exact f; exact Float32.zero.
+}
+{
+subst.
+destruct (Maps.PTree.get i m); [ | exact Float.zero].
+destruct v; try exact f; exact Float.zero.
+}
+exact (B754_zero (fprec ty) (femax ty) false).
+Defined.
+
+Ltac unfold_reflect E := 
+match goal with |- context [fval (list_to_env ?L) E] =>
+ pattern (fval (list_to_env L) E);
+ let HIDE := fresh "HIDE" in match goal with |- ?A _ => set (HIDE:=A) end;
+ let m := fresh "m" in let m' := fresh "m'" in
+ set (m := list_to_env L);
+ hnf in m;
+ set (m' := (Maps.PTree_Properties.of_list L)) in m;
+ hnf in m'; simpl in m';
+ let e' := eval hnf in E in change E with e';
+ cbv [fval type_of_expr type_of_unop Datatypes.id];
+ repeat change (type_lub _ _) with Tsingle;
+ repeat change (type_lub _ _) with Tdouble;
+ repeat change (cast_lub_l Tsingle Tsingle ?x) with x;
+ repeat change (cast_lub_r Tsingle Tsingle ?x) with x;
+ repeat change (cast_lub_l Tdouble Tdouble ?x) with x;
+ repeat change (cast_lub_r Tdouble Tdouble ?x) with x;
+ cbv [fop_of_unop fop_of_exact_unop fop_of_binop fop_of_rounded_binop];
+ change (BOPP Tsingle) with Float32.neg;
+ change (BPLUS Tsingle) with Float32.add;
+ change (BMULT Tsingle) with Float32.mul;
+ change (BDIV Tsingle) with Float32.div;
+ repeat match goal with |- context [m ?t ?i] =>
+             let u := fresh "u" in set (u := m t i); hnf in u; subst u
+ end;
+ subst m' m;
+ subst HIDE; cbv beta
+end.
 
 
 
